solve those 2 admits

src/cddl/pulse/CDDL.Pulse.Serialize.MapGroup2.fst
@@ -483,7 +483,7 @@ module Map = CDDL.Spec.Map
 #push-options "--z3rlimit 32 --split_queries always"
 
 #restart-solver
-let map_of_list_is_append_serializable_disjoint
+let map_of_list_serializable_disjoint
   (#key #value: Type)
   (#tkey: typ)
   (sp1: spec tkey key true)
@@ -493,11 +493,7 @@ let map_of_list_is_append_serializable_disjoint
   (except: map_constraint { inj \/ map_constraint_value_injective tkey sp2.parser except })
   (m1: Map.t key (list value))
   (m2: Map.t key (list value))
-  (m: Map.t key (list value))
 : Lemma
-  (requires (
-    map_of_list_is_append m1 m2 m
-  ))
   (ensures (
     let sp = mg_zero_or_more_match_item sp1 sp2 except in
     (sp.mg_serializable m1 /\ sp.mg_serializable m2) ==>
@@ -581,7 +577,7 @@ let map_of_list_is_append_serializable_intro
   ))
 = let sp = mg_zero_or_more_match_item sp1 sp2 except in
   map_of_list_is_append_serializable_intro_serializable sp1 sp2 except m1 m2 m;
-  map_of_list_is_append_serializable_disjoint sp1 sp2 except m1 m2 m;
+  map_of_list_serializable_disjoint sp1 sp2 except m1 m2;
   if sp.mg_serializable m1 && sp.mg_serializable m2 && cbor_map_disjoint_tot (sp.mg_serializer m1) (sp.mg_serializer m2)
   then begin
     assert (
@@ -658,7 +654,7 @@ let map_of_list_is_append_serializable_elim
       sp.mg_serializable m2 /\
       Map.disjoint m1 m2
     );
-    map_of_list_is_append_serializable_disjoint sp1 sp2 except m1 m2 m
+    map_of_list_serializable_disjoint sp1 sp2 except m1 m2
   end
 
 let map_of_list_is_append_serializable_elim'
@@ -785,7 +781,7 @@ let impl_serialize_map_group_valid_map_zero_or_more_snoc_aux
   map_of_list_is_append_serializable_singleton sp1 sp2 except k (key_eq k) v;
   let sp = mg_zero_or_more_match_item sp1 sp2 except in
   map_of_list_is_append_serializable_intro sp1 sp2 except m1 mkv m1';
-  map_of_list_is_append_serializable_disjoint sp1 sp2 except m1 mkv m1';
+  map_of_list_serializable_disjoint sp1 sp2 except m1 mkv;
   if
         sp1.serializable k &&
         sp2.serializable v &&
@@ -850,7 +846,7 @@ let impl_serialize_map_group_valid_map_zero_or_more_snoc1
   map_of_list_is_append_serializable_elim sp1 sp2 except mkv m2 m2';
   map_of_list_is_append_serializable_singleton sp1 sp2 except k (key_eq k) v;
   map_of_list_is_append_serializable_intro sp1 sp2 except m1 mkv m1';
-  map_of_list_is_append_serializable_disjoint sp1 sp2 except m1 mkv m1';
+  map_of_list_serializable_disjoint sp1 sp2 except m1 mkv;
   assert (sp1.serializable k);
   assert (sp2.serializable v);
   assert (~ (except (sp1.serializer k, sp2.serializer v)));
@@ -917,10 +913,10 @@ let impl_serialize_map_group_valid_map_zero_or_more_snoc2
   assert (~ (cbor_map_defined (sp1.serializer k) (sp.mg_serializer m1)));
   map_of_list_is_append_snoc key_eq m1 k v;
   map_of_list_is_append_serializable_intro sp1 sp2 except m1 mkv m1';
-  map_of_list_is_append_serializable_disjoint sp1 sp2 except m1 mkv m1';
+  map_of_list_serializable_disjoint sp1 sp2 except m1 mkv;
   map_of_list_is_append_serializable_singleton sp1 sp2 except k (key_eq k) v;
   map_of_list_is_append_serializable_elim sp1 sp2 except mkv m2 m2';
-  map_of_list_is_append_serializable_disjoint sp1 sp2 except mkv m2 m2';
+  map_of_list_serializable_disjoint sp1 sp2 except mkv m2;
   map_of_list_is_append_serializable_intro sp1 sp2 except mkv m2 m2';
             let ll = cbor_map_length l in
             cbor_map_length_disjoint_union (sp.mg_serializer m1) (sp.mg_serializer mkv);
@@ -979,6 +975,113 @@ let map_of_list_maps_to_nonempty_cons
   (map_of_list_maps_to_nonempty (map_of_list_cons k_eq k v m))
 = ()
 
+#push-options "--z3rlimit 32"
+
+#restart-solver
+let impl_serialize_map_group_valid_map_zero_or_more_snoc_disjoint1
+  (#key #value: Type)
+  (#tkey: typ)
+  (sp1: spec tkey key true)
+  (key_eq: EqTest.eq_test key)
+  (#tvalue: typ)
+  (#inj: bool)
+  (sp2: spec tvalue value inj)
+  (except: map_constraint { inj \/ map_constraint_value_injective tkey sp2.parser except })
+  (l: cbor_map)
+  (m1: Map.t key (list value))
+  (k: key)
+  (v: value)
+  (m2: Map.t key (list value))
+  (sq: squash (
+    let sp = mg_zero_or_more_match_item sp1 sp2 except in
+    sp.mg_serializable m1 /\
+    sp1.serializable k /\
+    sp2.serializable v /\
+    (~ (except (sp1.serializer k, sp2.serializer v))) /\
+    sp.mg_serializable m2 /\
+    (~ (Map.defined k m2)) /\
+    (~ (cbor_map_defined (sp1.serializer k) (cbor_map_union l (sp.mg_serializer m1))))
+  ))
+: Tot (squash (
+    let sp = mg_zero_or_more_match_item sp1 sp2 except in
+    let m1' = map_of_list_snoc key_eq m1 k v in    
+    sp.mg_serializable m1' /\
+    cbor_map_disjoint (sp.mg_serializer m1') (sp.mg_serializer m2) <==> cbor_map_disjoint (sp.mg_serializer m1) (sp.mg_serializer m2)
+  ))
+= 
+  let mkv = EqTest.map_singleton k (key_eq k) [v] in
+  map_of_list_maps_to_nonempty_singleton k (key_eq k) [v] ();
+  let m1' = map_of_list_snoc key_eq m1 k v in
+  map_of_list_is_append_snoc key_eq m1 k v;
+  map_of_list_is_append_serializable_intro sp1 sp2 except m1 mkv m1';
+  map_of_list_serializable_disjoint sp1 sp2 except m1 mkv;
+  map_of_list_serializable_disjoint sp1 sp2 except m1 m2;
+  map_of_list_serializable_disjoint sp1 sp2 except m1' m2;
+  ()
+
+#restart-solver
+let impl_serialize_map_group_valid_map_zero_or_more_snoc_length1
+  (#key #value: Type)
+  (#tkey: typ)
+  (sp1: spec tkey key true)
+  (key_eq: EqTest.eq_test key)
+  (#tvalue: typ)
+  (#inj: bool)
+  (sp2: spec tvalue value inj)
+  (except: map_constraint { inj \/ map_constraint_value_injective tkey sp2.parser except })
+  (l: cbor_map)
+  (m1: Map.t key (list value))
+  (k: key)
+  (v: value)
+  (m2: Map.t key (list value))
+  (sq: squash (
+    let sp = mg_zero_or_more_match_item sp1 sp2 except in
+    let m2' = map_of_list_cons key_eq k v m2 in
+    sp.mg_serializable m1 /\
+    cbor_map_disjoint l (sp.mg_serializer m1) /\
+    map_of_list_maps_to_nonempty m2 /\
+    sp1.serializable k /\
+    sp2.serializable v /\
+    (~ (except (sp1.serializer k, sp2.serializer v))) /\
+    sp.mg_serializable m2 /\
+    (~ (Map.defined k m2)) /\
+    (~ (cbor_map_defined (sp1.serializer k) (cbor_map_union l (sp.mg_serializer m1)))) /\
+    sp.mg_serializable m2' /\
+    cbor_map_disjoint (cbor_map_union l (sp.mg_serializer m1)) (sp.mg_serializer m2')
+  ))
+: Tot (squash (
+    let sp = mg_zero_or_more_match_item sp1 sp2 except in
+    let m1' = map_of_list_snoc key_eq m1 k v in    
+    let m2' = map_of_list_cons key_eq k v m2 in
+    sp.mg_serializable m1' /\
+    sp.mg_serializable m2' /\
+    cbor_map_length (cbor_map_union l (sp.mg_serializer m1)) + cbor_map_length (sp.mg_serializer m2') == cbor_map_length (cbor_map_union l (sp.mg_serializer m1')) + cbor_map_length (sp.mg_serializer m2)
+  ))
+= 
+  impl_serialize_map_group_valid_map_zero_or_more_snoc_disjoint1 sp1 key_eq sp2 except l m1 k v m2 ();
+  let mkv = EqTest.map_singleton k (key_eq k) [v] in
+  map_of_list_maps_to_nonempty_singleton k (key_eq k) [v] ();
+  let m1' = map_of_list_snoc key_eq m1 k v in
+  let m2' = map_of_list_cons key_eq k v m2 in
+  map_of_list_serializable_disjoint sp1 sp2 except m1' m2;
+  map_of_list_serializable_disjoint sp1 sp2 except m1 m2';
+  let sp = mg_zero_or_more_match_item sp1 sp2 except in
+  map_of_list_is_append_snoc key_eq m1 k v;
+  map_of_list_is_append_serializable_intro sp1 sp2 except m1 mkv m1';
+  map_of_list_is_append_cons key_eq k v m2;
+  map_of_list_is_append_serializable_intro sp1 sp2 except mkv m2 m2';
+  cbor_map_length_disjoint_union l (sp.mg_serializer m1');
+  let ll = cbor_map_length l in
+  cbor_map_length_disjoint_union (sp.mg_serializer m1) (sp.mg_serializer mkv);
+  let lm1 = cbor_map_length (sp.mg_serializer m1) in
+  cbor_map_length_disjoint_union l (sp.mg_serializer m1);
+  cbor_map_length_disjoint_union (sp.mg_serializer mkv) (sp.mg_serializer m2);
+  let lm2 = cbor_map_length (sp.mg_serializer m2) in
+  impl_serialize_map_group_valid_map_zero_or_more_snoc_length ll lm1 1 lm2;
+  ()
+
+#pop-options
+
 #push-options "--z3rlimit 128 --z3cliopt 'smt.qi.eager_threshold=100' --print_implicits --split_queries always"
 
 #restart-solver
@@ -1031,7 +1134,7 @@ let impl_serialize_map_group_valid_map_zero_or_more_snoc'
   map_of_list_is_append_serializable_singleton sp1 sp2 except k (key_eq k) v;
   let sp = mg_zero_or_more_match_item sp1 sp2 except in
   map_of_list_is_append_serializable_intro sp1 sp2 except m1 mkv m1';
-  map_of_list_is_append_serializable_disjoint sp1 sp2 except m1 mkv m1';
+  map_of_list_serializable_disjoint sp1 sp2 except m1 mkv;
   if
     sp1.serializable k &&
     sp2.serializable v &&
@@ -1039,7 +1142,7 @@ let impl_serialize_map_group_valid_map_zero_or_more_snoc'
   then begin
     if sp.mg_serializable m2
     then begin
-      map_of_list_is_append_serializable_disjoint sp1 sp2 except mkv m2 m2';
+      map_of_list_serializable_disjoint sp1 sp2 except mkv m2;
       if Map.defined k m2
       then ()
       else begin
@@ -1055,19 +1158,14 @@ let impl_serialize_map_group_valid_map_zero_or_more_snoc'
           assert (cbor_map_disjoint l (sp.mg_serializer m2') <==> cbor_map_disjoint l (sp.mg_serializer m2));
           assert (cbor_map_disjoint (sp.mg_serializer m1) (sp.mg_serializer m2') <==> cbor_map_disjoint (sp.mg_serializer m1) (sp.mg_serializer m2));
           map_of_list_is_append_snoc key_eq m1 k v;
-          assume (cbor_map_disjoint (sp.mg_serializer m1') (sp.mg_serializer m2) <==> cbor_map_disjoint (sp.mg_serializer m1) (sp.mg_serializer m2));
+          impl_serialize_map_group_valid_map_zero_or_more_snoc_disjoint1 sp1 key_eq sp2 except l m1 k v m2 ();
+          assert (cbor_map_disjoint (sp.mg_serializer m1') (sp.mg_serializer m2) <==> cbor_map_disjoint (sp.mg_serializer m1) (sp.mg_serializer m2));
           assert (cbor_map_disjoint (cbor_map_union l (sp.mg_serializer m1)) (sp.mg_serializer m2') <==> cbor_map_disjoint (cbor_map_union l (sp.mg_serializer m1')) (sp.mg_serializer m2));
           if cbor_map_disjoint_tot (cbor_map_union l (sp.mg_serializer m1)) (sp.mg_serializer m2')
           then begin
             cbor_map_length_disjoint_union l (sp.mg_serializer m1');
-            let ll = cbor_map_length l in
-            cbor_map_length_disjoint_union (sp.mg_serializer m1) (sp.mg_serializer mkv);
-            let lm1 = cbor_map_length (sp.mg_serializer m1) in
-            cbor_map_length_disjoint_union l (sp.mg_serializer m1);
-            cbor_map_length_disjoint_union (sp.mg_serializer mkv) (sp.mg_serializer m2);
-            let lm2 = cbor_map_length (sp.mg_serializer m2) in
-            impl_serialize_map_group_valid_map_zero_or_more_snoc_length ll lm1 1 lm2;
-            assume (cbor_map_length (cbor_map_union l (sp.mg_serializer m1)) + cbor_map_length (sp.mg_serializer m2') == cbor_map_length (cbor_map_union l (sp.mg_serializer m1')) + cbor_map_length (sp.mg_serializer m2));
+            impl_serialize_map_group_valid_map_zero_or_more_snoc_length1 sp1 key_eq sp2 except l m1 k v m2 ();
+            assert (cbor_map_length (cbor_map_union l (sp.mg_serializer m1)) + cbor_map_length (sp.mg_serializer m2') == cbor_map_length (cbor_map_union l (sp.mg_serializer m1')) + cbor_map_length (sp.mg_serializer m2));
             assert (cbor_map_length (cbor_map_union l (sp.mg_serializer m1)) + cbor_map_length (sp.mg_serializer m2') >= cbor_map_length (cbor_map_union l (sp.mg_serializer m1)) + 1);
             let sl = Seq.length (Cbor.cbor_det_serialize_map l) in
             let sm1 = Seq.length (Cbor.cbor_det_serialize_map (sp.mg_serializer m1)) in
